updated with testing on knows predicate

SecurityNotation/Logic/logic.lean
@@ -1,7 +1,17 @@
-import SecurityNotation.Basic.Syntax
+import SecurityNotation.Basic.Syntax.Principal
+import SecurityNotation.Basic.Syntax.Messages
+import SecurityNotation.Basic.Syntax.Keys
+
 
 -- I will write this whilst i do my proofs as I do not know what i will need just yet
 
 -- define the logic for the security notation
 -- need predicates: Knows, Honest, Fresh, Compromised, Trusted,
---def knows (a : Principal) (m : Message) : Prop :=
+-- def knows (a : Principal) (m : Message) : Prop :=
+
+-- based on the Dolev-Yao Model
+inductive knows (initial_knowledge : Principal → Message → Prop) : Principal → Message → Prop where
+  | base : ∀ p m, initial_knowledge p m → knows initial_knowledge p m
+  | pair_unpack_l : ∀ p m1 m2, knows initial_knowledge p (Message.pair m1 m2) → knows initial_knowledge p m1
+  | pair_unpack_r : ∀ p m1 m2, knows initial_knowledge p (Message.pair m1 m2) → knows initial_knowledge p m2
+  | decrypt : ∀ p m k, knows initial_knowledge p (Message.enc m k) → knows initial_knowledge p (Message.key k) → knows initial_knowledge p m
