SecurityNotation/Testing/initialTesting.lean
@@ -2,6 +2,7 @@ import SecurityNotation.Basic.Syntax.Principal
 import SecurityNotation.Basic.Syntax.Nonces
 import SecurityNotation.Basic.Syntax.Keys
 import SecurityNotation.Basic.Syntax.Messages
+import SecurityNotation.Logic.Logic
 
 -- testing the imports in lean
 
@@ -15,13 +16,16 @@ def same (a b : Principal) : Bool :=
 #eval same (Principal.mk 1 "Alice" Role.responder) (Principal.mk 1 "Alice" Role.responder)
 #eval same (Principal.mk 1 "Bob" Role.responder) (Principal.mk 1 "Alice" Role.responder)
 
-def exampleB : IO Unit := do
+def example_b : IO Unit := do
   let mynonce ← Nonce.fresh
   IO.println s!"my fresh nonce is {mynonce.randomNum} and {mynonce.timestamp}"
   IO.println "--------------------------------"
   IO.println s!"my fresh nonce is {mynonce.randomNum} and {mynonce.timestamp}"
-#eval exampleB
+#eval example_b
 
+--testing the messages
+
+-- message encoding a message to a principal using a public key
 def message1 (a1 : String) (alice : Principal) (pKb : Key) : Message :=
   Message.enc (Message.pair (Message.message a1) (Message.agent alice)) pKb
 
@@ -29,3 +33,40 @@ def alice : Principal := {id := 1,name := "Alice",role :=  Role.initiator}
 def keyA : Key := Key.new 1 keyType.publicKey (some alice) []
 
 #eval message1 "hello world!" alice keyA
+
+--testing knows logic from logic.lean
+
+variable (kb : Principal → Message → Prop)
+
+theorem alice_knows (alice : Principal) (m : Message) :
+  kb alice m → knows kb alice m := by
+  apply knows.base
+
+--testing for alice_decrypts
+--creating a private key for alice
+def alice_priv_key : Key :=
+  Key.new 1 keyType.publicKey (some alice) [alice]
+--creating the knowledge base for what alie konws and can draw from
+def kb_decrypt (p : Principal) (m : Message) : Prop :=
+  match p.name with
+  | "alice" =>
+    m = Message.key alice_priv_key
+  | _ => False
+
+theorem alice_decrypt (p: Principal) (m : Message) :
+  p.name = "alice" → knows kb_decrypt p (Message.enc m alice_priv_key) → knows kb_decrypt p m := by
+  intro h_name h_enc_m
+  apply knows.decrypt p m alice_priv_key
+  . exact h_enc_m
+  · apply knows.base
+    unfold kb_decrypt
+    rw [h_name]
+    simp
+
+#check alice_decrypt
+
+#check alice_knows
+
+#check knows.base
+
+#check knows.decrypt
